code/chacha20poly1305/Hacl.Impl.Chacha20Poly1305.PolyCore.fst
@@ -15,7 +15,6 @@ module Spec = Spec.Chacha20Poly1305
 module Poly = Hacl.Impl.Poly1305
 open Hacl.Impl.Poly1305.Fields
 open Hacl.Spec.Poly1305.Equiv
-open Hacl.Impl.Chacha20Poly1305.PolyLemmas
 
 #set-options "--z3rlimit 50 --max_fuel 0 --max_ifuel 0"
 
@@ -34,7 +33,7 @@ let poly1305_padded ctx len text tmp =
   let h1 = ST.get() in
   update_sub tmp 0ul r rem;
   let h2 = ST.get() in
-  same_ctx_same_r_acc ctx h1 h2;
+  Poly.reveal_ctx_inv ctx h1 h2;
   update1_equiv (Poly.as_get_r h2 ctx) 16 (as_seq h2 tmp) (Poly.as_get_acc h2 ctx);  
   Poly.poly1305_update ctx 16ul tmp
 
